Isabelle/Shelley/Protocol_Parameters.thy
@@ -1,7 +1,7 @@
 section \<open> Protocol Parameters \<close>
 
 theory Protocol_Parameters
-  imports "HOL.Complex" Finite_Map_Extras
+  imports "HOL.Complex" Finite_Map_Extras Basic_Types
 begin
 
 text \<open> Protocol parameter name \<close>
@@ -18,6 +18,12 @@ type_synonym p_params = "(ppm, pvalue) fmap"
 
 text \<open> Accessor Functions \<close>
 
+consts max_block_size :: "p_params \<Rightarrow> nat" \<comment> \<open>max block body size\<close>
+
+consts max_tx_size :: "p_params \<Rightarrow> nat" \<comment> \<open>max transaction size\<close>
+
+consts max_header_size :: "p_params \<Rightarrow> nat" \<comment> \<open>max block header size\<close>
+
 consts tau :: "p_params \<Rightarrow> real" \<comment> \<open>[0, 1]\<close>
 
 consts rho :: "p_params \<Rightarrow> real" \<comment> \<open>[0, 1]\<close>
@@ -27,5 +33,10 @@ consts active_slot_coeff :: "p_params \<Rightarrow> real" \<comment> \<open>[0, 
 text \<open> Global Constants \<close>
 
 consts slots_per_epoch :: nat
+
+text \<open> Helper Functions \<close>
+
+fun first_slot :: "epoch \<Rightarrow> slot" where
+  "first_slot e = undefined" \<comment> \<open>NOTE: Undefined for now\<close>
 
 end
